restore lifting lemmas

lexical.dfy
@@ -20,10 +20,47 @@ module Lexical_Order_Strings refines Total_Order {
 		else ltedef(a[1..], b[1..])
 	}
 
-  lemma ltedef_properties(a: Element, b: Element)
+    lemma ltedef_properties(a: Element, b: Element)
 		ensures ltedef(a, b) || ltedef(b, a); // Total
 		ensures ltedef(a, b) && ltedef(b, a) ==> a == b; // Antisymmetric
-  {
-  }
+    {
+    }
 
+    function method longest_common_prefix<T(==)>(a: seq<T>, b: seq<T>) : seq<T>
+        ensures longest_common_prefix<T>(a, b) <= a;
+        ensures longest_common_prefix<T>(a, b) <= b;
+        ensures
+            |longest_common_prefix<T>(a, b)| == |a| ||
+            |longest_common_prefix<T>(a, b)| == |b| ||
+            a[|longest_common_prefix<T>(a, b)|] != b[|longest_common_prefix<T>(a, b)|];
+    {
+        if |a| == 0 || |b| == 0 || a[0] != b[0] then []
+        else [a[0]] + longest_common_prefix<T>(a[1..], b[1..])
+    }
+
+    lemma lexical_cmp_between_implies_common_prefix(a: string, b: string, c: string)
+        requires lte(a, b);
+        requires lte(b, c);
+        ensures
+            longest_common_prefix<char>(a, c) == longest_common_prefix<char>(a, b) ||
+            longest_common_prefix<char>(a, c) == longest_common_prefix<char>(b, c);
+    {
+        if |longest_common_prefix<char>(a, c)| > 0 {
+            assert a[0] == b[0] && b[0] == c[0];
+            lexical_cmp_between_implies_common_prefix(a[1..], b[1..], c[1..]);
+        }
+    }
+
+    lemma lexical_cmp_between_implies_common_prefix_forall()
+        ensures forall a, b, c :: lte(a, b) && lte(b, c) ==>
+        longest_common_prefix<char>(a, c) == longest_common_prefix<char>(a, b) ||
+        longest_common_prefix<char>(a, c) == longest_common_prefix<char>(b, c);
+    {
+    }
+
+  
 }
+
+// Local Variables:
+// tab-width: 4
+// End:
